exp/map.lean: rewrite with pattern matching

src/exp/map.lean
@@ -17,86 +17,25 @@ variables {p : X ⊆ Y} {q : Y ⊆ Z} -- Subset properties
 
 -- Given proof `p : X ⊆ Y`, `map p e` maps the free variables from `X` to `Y` in
 -- `e : exp X`.
-def map : X ⊆ Y → exp X → exp Y :=
-  begin
-    intros p e,
-    induction e with
-      /- var -/ X x
-      /- app -/ X f e rf re
-      /- lam -/ X x e r
-      generalizing Y p,
-    begin /- var -/
-      exact var (vname.map_of_subset p x)
-    end,
-    begin /- app -/
-      exact app (rf p) (re p)
-    end,
-    begin /- lam -/
-      exact lam (r $ vset.prop_insert_of_subset x p)
-    end
-  end
+def map : ∀ {X Y : vs V}, X ⊆ Y → exp X → exp Y
+  | X Y p (var x)              := var (vname.map_of_subset p x)
+  | X Y p (app f e)            := app (map p f) (map p e)
+  | X Y p (@lam _ _ _ _ _ a e) := lam (map (vset.prop_insert_of_subset a p) e)
 
 namespace map ------------------------------------------------------------------
 
 -- Identity of `map`.
-theorem id (e : exp X) : map (vset.prop_subset_refl X) e = e :=
-  begin
-    induction e with
-      /- var -/ X x
-      /- app -/ X e₁ e₂ r₁ r₂
-      /- lam -/ X x e r,
-    begin /- var -/
-      cases x,
-      reflexivity
-    end,
-    begin /- app -/
-      conv {to_rhs, rw [←r₁, ←r₂]},
-      reflexivity
-    end,
-    begin /- lam -/
-      conv {to_rhs, rw [←r]},
-      reflexivity
-    end
-  end
-
-/-
-Useful equalities for targeted rewriting.
--/
-
-theorem of_var (x : ν∈ X)
-: map p (var x) = var (vname.map_of_subset p x) :=
-  rfl
-
-theorem of_app (f e : exp X)
-: map p (app f e) = app (map p f) (map p e) :=
-  rfl
-
-theorem of_lam (e : exp (insert a X))
-: map p (lam e) = lam (map (vset.prop_insert_of_subset a p) e) :=
-  rfl
+theorem id : ∀ {X : vs V} (e : exp X), e = map (vset.prop_subset_refl X) e
+  | X (var x)   := by cases x; reflexivity
+  | X (app f e) := by rw map; conv {to_lhs, rw [id f, id e]}
+  | X (lam e)   := by rw map; conv {to_lhs, rw [id e]}; reflexivity
 
 -- Composition of `map`.
-theorem comp (e : exp X)
-: map q (map p e) = map (vset.prop_subset_trans p q) e :=
-  begin
-    induction e with
-      /- var -/ X x
-      /- app -/ X f e rf re
-      /- lam -/ X x e r
-      generalizing Y Z p q,
-    begin /- var -/
-      repeat {rw [map.of_var]}
-    end,
-    begin /- app -/
-      repeat {rw [map.of_app]},
-      rw [rf, re]
-    end,
-    begin /- lam -/
-      repeat {rw [map.of_lam]},
-      rw [r],
-      reflexivity
-    end
-  end
+theorem comp : ∀ {X Y Z : vs V} {p : X ⊆ Y} {q : Y ⊆ Z} (e : exp X),
+map q (map p e) = map (vset.prop_subset_trans p q) e
+  | X Y Z p q (var x)   := by repeat {rw [map]}
+  | X Y Z p q (app f e) := by repeat {rw [map]}; rw [comp f, comp e]
+  | X Y Z p q (lam e)   := by repeat {rw [map]}; rw [comp e]; reflexivity
 
 end /- namespace -/ map --------------------------------------------------------
 
@@ -107,35 +46,9 @@ def insert_var (a : V) : exp X → exp (insert a X) :=
 
 namespace insert_var -----------------------------------------------------------
 
-/-
-Useful equalities for targeted rewriting.
--/
-
-theorem of_var (x : ν∈ X)
-: insert_var a (var x) = var (vname.insert a x) :=
-  rfl
-
-theorem of_app (f e : exp X)
-: insert_var a (app f e) = app (insert_var a f) (insert_var a e) :=
-  rfl
-
-theorem of_lam₁ (e : exp (insert a X))
-: insert_var b (lam e) = lam (map (vset.prop_insert_of_subset a (vset.prop_subset_insert_self b X)) e) :=
-  rfl
-
-theorem of_lam₂ (e : exp (insert a X))
+theorem lam_comp (e : exp (insert a X))
 : insert_var b (lam e) = lam (map (vset.prop_subset_of_insert_comm b a X) (insert_var b e)) :=
-  begin
-    unfold insert_var,
-    rw [map.comp e],
-    reflexivity
-  end
-
-theorem of_lam₃ (e : exp (insert a X))
-: insert_var (fresh X).1 (lam e) = lam (map (vset.prop_subset_of_insert_comm (fresh X).1 a X) (insert_var (fresh X).1 e)) :=
-  begin
-    exact of_lam₂ e
-  end
+  by unfold insert_var; rw [map.comp e]; reflexivity
 
 end /- namespace -/ insert_var -------------------------------------------------
 
